% SampleProject.tex -- main LaTeX file for sample LaTeX article
%
%\documentclass[12pt]{article}
\documentclass[11pt]{SelfArxOneColBMN}
% add the pgf and tikz support.  This automatically loads
% xcolor so no need to load color
\usepackage{pgf}
\usepackage{tikz}
\usetikzlibrary{matrix}
\usetikzlibrary{calc}
\usepackage{xstring}
\usepackage{pbox}
\usepackage{etoolbox}
\usepackage{marginfix}
\usepackage{xparse}
\setlength{\parskip}{0pt}% fix as marginfix inserts a 1pt ghost parskip
% standard graphics support
\usepackage{graphicx,xcolor}
\usepackage{wrapfig}
%
\definecolor{color1}{RGB}{0,0,90} % Color of the article title and sections
\definecolor{color2}{RGB}{0,20,20} % Color of the boxes behind the abstract and headings
%----------------------------------------------------------------------------------------
% HYPERLINKS
%----------------------------------------------------------------------------------------
\usepackage[pdftex]{hyperref} % Required for hyperlinks
\hypersetup{hidelinks,
colorlinks,
breaklinks=true,%
urlcolor=color2,%
citecolor=color1,%
linkcolor=color1,%
bookmarksopen=false%
,pdftitle={SampleProject},%
pdfauthor={Peterson}}
%\usepackage[round,numbers]{natbib}
\usepackage[numbers]{natbib}
\usepackage{lmodern}
\usepackage{setspace}
\usepackage{xspace}
%
\usepackage{subfigure}
\newcommand{\goodgap}{
  \hspace{\subfigtopskip}
  \hspace{\subfigbottomskip}}
%
\usepackage{atbegshi}
%
\usepackage[hyper]{listings}
%
% use ams math packages
\usepackage{amsmath,amsthm,amssymb,amsfonts}
\usepackage{mathrsfs}
%
% use new improved Verbatim
\usepackage{fancyvrb}
%
\usepackage[titletoc,title]{appendix}
%
\usepackage{url}
%
% Create length for the baselineskip of text in footnotesize
\newdimen\footnotesizebaselineskip
\newcommand{\test}[1]{%
 \setbox0=\vbox{\footnotesize\strut Test \strut}
 \global\footnotesizebaselineskip=\ht0 \global\advance\footnotesizebaselineskip by \dp0
}
%
\usepackage{listings}

\DeclareGraphicsExtensions{.pdf, .jpg, .tif,.png}

% make sure we don't get orphaned words if at top of page
% or orphans if at bottom of page
\clubpenalty=9999
\widowpenalty=9999
\renewcommand{\textfraction}{0.15}
\renewcommand{\topfraction}{0.85}
\renewcommand{\bottomfraction}{0.85}
\renewcommand{\floatpagefraction}{0.66}
%
\DeclareMathOperator{\sech}{sech}

\input{setupsample}

\JournalInfo{MATH 8210:  E-Learning Homework, 1-\pageref{LastPage}, 2020} % Journal information
\Archive{Draft Version \today} % Additional notes (e.g. copyright, DOI, review/research article)

\PaperTitle{MATH 8210 E-Learning Homework}
\Authors{Ian Davis\textsuperscript{1}}
\affiliation{\textsuperscript{1}\textit{John E. Walker Department of Economics,
Clemson University,Clemson, SC: email ijdavis@g.clemson.edu}}
%\affiliation{*\textbf{Corresponding author}: yournamehere@clemson.edu} % Corresponding author

\date{\small{Version ~\today}}
\Abstract{Variation of Parameters and Boundry Value Problems}
\Keywords{}
\newcommand{\keywordname}{Keywords}
%
\onehalfspacing
\begin{document}

\flushbottom
\addcontentsline{toc}{section}{Title}
\maketitle

\renewcommand{\theexercise}{\arabic{exercise}}%

\noindent Use VoP to solve

\begin{exercise}
  Consider
  \begin{eqnarray*}
    u''(t) - 4u(t) &=& f(t)\\
    u(0) &=& 1\\
    u(8) &=& -1\\
  \end{eqnarray*}
  where f is a continuous function
  \begin{solution}
    In this case, we want to note that we can follow the usual VoP steps with $\beta^2 = 1$. So this means that
    \begin{eqnarray*}
      4x_p(t) &=& v_1(t)e^{-t} + v_2(t)e^{t}\\
      4x_p'(t) &=& v_1'(t)e^{-t} - v_1(t)e^{-t} + v_2(t)e^{t} + v_2(t)e^{-t}\\
      &=& (v_1'(t)e^{-t} + v_2'(t)e^{t}) + (-v_1(t)e^{-t} + v_2(t)e^{-t})
    \end{eqnarray*}
    Now, we consider the related system
    \begin{eqnarray*}
      \frac{1}{4}
      \begin{bmatrix}
        e^{-t} & e^t \\
        -e^{-t} & e^t
      \end{bmatrix}
      \begin{bmatrix}
        \phi(t) \\
        \psi(t)
      \end{bmatrix}
      &=&
      \begin{bmatrix}
        0 \\
        f(t)
      \end{bmatrix}
      \\
      \implies \frac{1}{4}(v_1'(t)e^{-t} + v_2'(t)e^t) &=& 0\\
    \end{eqnarray*}
    as well as
    \begin{eqnarray*}
      x'p(t) = \frac{1}{4}(-v_1(t)e^{-t} + v_2(t)e^t) = 0\\
      \implies x_p''(t) = \frac{1}{4}(-v_1'(t)e^{-t} + v_2'(t)e^t + v_1(t)e^{-t} + v_2(t)e^t)
    \end{eqnarray*}
    Plugging this in to the nonhomogenous equation we get
    \begin{eqnarray*}
      f(t) &=& \frac{1}{4}(v_2'(t)e^t - v_1'(t)e^{-t} + v_2(t)e^t + v_1(t)e^{-t} - (v_2(t)e^t + v_1(t)e^{-t}))\\
      \implies f(t) &=& \frac{1}{4}(v_2'(t)e^t - v_1'(t)e^t)
    \end{eqnarray*}
    Then, by Cramer's rule, we get
    \begin{eqnarray*}
      v_1'(t) &=& -2f(t)e^t = -2f(t)e^t\\
      v_2'(t) &=& 2f(t)e^{-t} = 2f(t)e^{-t}\\
    \end{eqnarray*}
    which imply
    \begin{eqnarray*}
      v_1(t) &=& -2\int_0^t\:f(u)e^udu\\
      v_2(t) &=& 2\int_0^t\:f(u)e^{-u}du\\
      \implies x_p(t) &=& v_1(t)e^{-t} + v_2(t)e^t\\
      &=& (-2\int_0^t\:f(u)e^udu)e^{-t} + (2\int_0^t\:f(u)e^{-u}du)e^t
    \end{eqnarray*}
    And our general solution is
    \begin{eqnarray*}
      x(t) &=& x_h(t) + x_p(t)\\
      &=& A_1e^{-t} + A_2e^t - 2e^{-t}\int_0^t\:f(u)e^udu + 2e^t\int_0^t\:f(u)e^{-u}du\\
      &=& A_1e^{-t} + A_2e^t - 2\int_0^t\:f(u)e^{u -t}du + 2\int_0^t\:f(u)e^{-(u -t)}du\\
      &=& A_1e^{-t} + A_2e^t + 2\int_0^t\:f(u)(e^{u - t} - e^{-(u - t)})\\
      &=& A_1cosh(t) + A_2sinh(t) + 2\int_0^1\:f(u)sinh(t - u)
    \end{eqnarray*}
    Now, we consider the two initial conditions
    \begin{eqnarray*}
      u(0) &=& 1\\
      \implies A_1 &=& 1
    \end{eqnarray*}
    and
    \begin{eqnarray*}
      U(8) &=& - 1\\
      \implies -1 &=& cosh(8) + A_2sinh(8) + 2\int_0^8\:f(u)sinh(8 - u)du\\
      \implies A_2 &=& -\frac{1}{sinh(8)}(cosh(8) + 2\int_0^8\:f(u)sinh(8 - u)du + 1)
    \end{eqnarray*}
  \end{solution}
\end{exercise}

\begin{exercise}
 Consider
  \begin{eqnarray*}
    u''(t) + 4u(t) &=& f(t)\\
    u(0) &=& 1\\
    u(6) &=& -1\\
  \end{eqnarray*}
  where f is a continuous function
  \begin{solution}
    The characterstic equation in this case is $r^2 + 4 = 0$ which has complex roots of $\pm 2i$. Hence $u_1(t) = cos(3t)$ and $u_2(t) = sin(3t)$ so we set the solution to be
    \begin{eqnarray*}
      u_p(t) = A(t)cos(2t) + B(t)sin(2t)
    \end{eqnarray*}
    and the nonhomogenous solution to be of the form
    \begin{eqnarray*}
      u_p(t) = \phi(t)cos(2t) + \psi(t)sin(2t)
    \end{eqnarray*}
    satisfying
    \begin{eqnarray*}
      \begin{bmatrix}
        cos(2t) & sin(2t) \\
        -2sin(2t) & 2cos(2t)
      \end{bmatrix}
      \begin{bmatrix}
        \phi'(t) \\
        \psi'(t)
      \end{bmatrix}
      &=&
      \begin{bmatrix}
        0 \\
        f(t)
      \end{bmatrix}
      \\
    \end{eqnarray*}
    Applying Cramer's rule we get
    \begin{eqnarray*}
      \phi'(t) = \frac{1}{2}
      \begin{vmatrix}
        0 & sin(2t) \\
        f(t) & 2cos(2t)
      \end{vmatrix}
      = -\frac{1}{2}f(t)sin(2t)
    \end{eqnarray*}
    and
    \begin{eqnarray*}
      \psi'(t) = \frac{1}{2}
      \begin{vmatrix}
        cos(2t) & 0 \\
        -2sin(2t) & f(t)
      \end{vmatrix}
      = \frac{1}{2}f(t)cos(2t)
    \end{eqnarray*}
    integrating gives us
    \begin{eqnarray*}
      \phi(t) &=& -\frac{1}{2}\int_0^t\: f(u)sin(2u)du\\
      \psi(t) &=& \frac{1}{2}\int_0^t\: f(u)cos(2u)du
    \end{eqnarray*}
    and the general solution is
    \begin{eqnarray*}
      u(t) &=& Acos(2t) + Bsin(2t) - \frac{1}{2}\int_0^t\: f(u)sin(2u)ducos(2t) + \frac{1}{2}\int_0^t\: cos(2u)dusin(2t)\\
      &=& Acos(2t) + Bsin(2t) + \frac{1}{2}\int_0^t\: f(u)sin(2t - 2u)du
    \end{eqnarray*}
    Now, considering the initial conditions we get
    \begin{eqnarray*}
      u(0) &=& 1\\
      \implies A &=& 1
    \end{eqnarray*}
    and
    \begin{eqnarray*}
      u(4) &=& -1\\
      \implies B &=& -\frac{1}{sin(8)}(cos(8) + \frac{1}{2}\int_0^4\: f(u)sin(8 - 2u)du + 1)
    \end{eqnarray*}
  \end{solution}
\end{exercise}

\noindent Do BVP analysis for
\begin{exercise}
 Consider
  \begin{eqnarray*}
    u'' + 9\omega^2u &=& f, \: 0 \leq x \leq 3,\\
    u'(0) &=& 0\\
    u'(3) &=& 0\\
  \end{eqnarray*}
\end{exercise}

\begin{solution}
  The general solution to the homogenous equaiton is given by
  \begin{eqnarray*}
    u_h(x) = Acos(3\omega x) + Bsin(3\omega x)
  \end{eqnarray*}
  Applying VoP gives
  \begin{eqnarray*}
    u_p(x) = \phi(x)cos(3\omega x) + \psi(x)sin(3\omega x)
  \end{eqnarray*}
  we want $\phi(x)$ and $\psi(x)$ which simplify
  \begin{eqnarray*}
    \begin{vmatrix}
      cos(3\omega x) & sin(3\omega x)\\
      -3\omega sin(3\omega x) & 3\omega cos(3\omega x)
    \end{vmatrix}
    \begin{vmatrix}
      \phi'(x)\\
      \psi'(x)
    \end{vmatrix}
    =
    \begin{vmatrix}
      0\\
      f(x)
    \end{vmatrix}
  \end{eqnarray*}
  The det of the 2x2 matrix above is $3\omega$ so we can use Cramer's rule to get
  \begin{eqnarray*}
    \phi'(x) = -\frac{f(x)sin(3\omega x)}{3\omega}\\
    \psi'(x) = \frac{f(x)cos(3\omega x)}{3\omega}
  \end{eqnarray*}
  Hence
  \begin{eqnarray*}
    \phi(x) = -\frac{1}{3\omega}\int_0^x\: f(s)sin(3\omega s)ds\\
    \psi(x) = \frac{1}{3\omega}\int_0^x\: f(s)cos(3\omega s)ds\\
  \end{eqnarray*}
  Because the general solution is
  \begin{eqnarray*}
    u(x) = u_n(x) + u_p(x)
  \end{eqnarray*}
  we get
  \begin{eqnarray*}
    u(x) = Acos(3\omega x) + Bsin(3\omega x) + \frac{1}{w}\int_0^x\: f(s)sin(3\omega(x - s))ds
  \end{eqnarray*}
  Next, we apply the boundary conditions. First, consider leibniez rule for derivatives which gives us
  \begin{eqnarray*}
    u'(x) = -3\omega Asin(3\omega x) + 3\omega cos(3\omega x) + \int_0^3\: f(s)cos(3\omega(3 - s))ds
  \end{eqnarray*}
  Hence, $u'(0) = 0 = 3\omega B$ and 
  \begin{eqnarray*}
    u'(3) &=& -3\omega Asin(9\omega) + 3\omega cos(9\omega) + \int_0^3\: f(s)cos(\omega(3 - s))\\
    \implies B &=& 0 
  \end{eqnarray*}
  But we cannot find A from 
  \begin{eqnarray*}
    0 = -3\omega Asin(9\omega) + 3\omega cos(9\omega) + \int_0^3\: f(s)cos(\omega(3 - s))\\
  \end{eqnarray*}
  So consider the cases.\\
  Case 1:
  \begin{eqnarray*}
    3\omega = n\pi \implies \int_0^3\: f(s)cos(n\pi(3 - s))ds = 0
  \end{eqnarray*}
  Case 2:
  \begin{eqnarray*}
    3\omega \neq n\pi\\
    \implies \frac{1}{3\omega sin(9\omega)}\int_0^3 \:f(s)cos(3\omega(3- s))ds = A
  \end{eqnarray*}
  giving us
  \begin{eqnarray*}
    u(x) = \frac{cos(3\omega x)}{3\omega sin(9\omega)}\int_0^3\: f(s)cos(3\omega(3 - s))ds + \frac{1}{3\omega}\int_0^x\: f(s)sin(3\omega(x - s))ds
  \end{eqnarray*}
  which can be manipulated to give us
  \begin{eqnarray*}
    u(x) = \int_0^3\: f(s)k_w(x,s)ds
  \end{eqnarray*}
  with
  \begin{eqnarray*}
    k_w(x,s) &=& \frac{1}{3\omega sin(9\omega)}
    \left \{
    \begin{array}{ll}
      cos(3\omega s)cos(3\omega(3 - x)), & 0 \leq s \leq x\\
      cos(3\omega x)cos(3\omega(3 - s)), & x < s \leq 3
    \end{array}
    \right
  \end{eqnarray*}
\end{solution}

\noindent Do the cable problem analysis for
\begin{exercise}
  \begin{eqnarray*}
    4\frac{\delta^2 \Phi}{\delta x^2} - \Phi - 0.7\frac{\delta\Phi}{\delta t} &=& 0, \: 0 \leq x \leq 6, \: t \geq 0,\\
    \frac{\delta\Phi}{\delta t}(0,t) &=& 0,\\
    \frac{\delta\Phi}{\delta t}(6,t) &=& 0,\\
    \Phi(x,0) &=& f(x)
  \end{eqnarray*}
  for $f(x) = 5x(6 - x)$. Find the first four terms of the solution $\Phi$.

  \begin{solution}
    Seperating the variables we get
    \begin{eqnarray*}
      \Phi(x,t) = u(x)w(t)
    \end{eqnarray*}
    giving us
    \begin{eqnarray*}
      4\frac{d^2u}{dx^2}w(t) - u(x)w(t) - .7u(x)\frac{dw}{dt} = 0 
    \end{eqnarray*}
    Rewriting we find, for all x,t we need
    \begin{eqnarray*}
      w(t)(4\frac{d^2u}{dx^2} - u(x)) = .7u(x)\frac{dw}{dt}
    \end{eqnarray*}
    Rewriting again, we have
    \begin{eqnarray*}
      \frac{4\frac{d^2u}{dx^2} - u(x)}{u(x)} = \frac{.7\frac{dw}{dt}}{w(t)}, 0 \leq x \leq 6, t > 0
    \end{eqnarray*}
    And get the following two conditions
    \begin{eqnarray*}
      .7\frac{dw}{dt} = \Theta w(t), t > 0\\
      4\frac{d^2u}{dx^2} = (1 + \Theta)u(x), 0 \leq x \leq 6
    \end{eqnarray*}
    We also get boundry conditions
    \begin{eqnarray*}
      \frac{du}{dx}(0)w(t) = 0, t > 0\\
      \frac{du}{dx}(6)w(t) = 0, t > 0
    \end{eqnarray*}
    Since these questions must hold for all t, it forces
    \begin{eqnarray*}
      \frac{du}{dx}(0) = 0\\
      \frac{du}{dx}(6) = 0
    \end{eqnarray*}
    The model now becomes
    \begin{eqnarray*}
      u'' - \frac{1 + \Theta}{4}u = 0\\
      \frac{du}{dx}(0) = 0\\
      \frac{du}{dx}(6) = 0
    \end{eqnarray*}
    We are only looking for nonzero solutions so any $\Theta$ leading to a zero gets rejected\\
    Case 1: $1 + \Theta = \omega^2, \omega \neq 0$
    \begin{eqnarray*}
      u'' - \frac{\omega^2}{4}u = 0\\
      u'(0) = 0\\
      u'(6) = 0
    \end{eqnarray*}
    with characteristic equation $r^2 - \frac{\omega^2}{4}$ with real roots $\pm \frac{\omega}{4}$. The general solution is given by $u(x) = Acosh(\frac{\omega}{2}x) + Bsinh(\frac{\omega}{2}x)$ which implies
    \begin{eqnarray*}
     u'(x) = A\frac{\omega}{2}sinh(\frac{\omega}{2}x) +  b\frac{\omega}{2}cosh(\frac{\omega}{2}x)
    \end{eqnarray*}
    Then apply the boundry conditions and get
    \begin{eqnarray*}
      u'(0) = B = 0\\
      u'(6) = 0 = Asinh(3\omega)
    \end{eqnarray*}
    But since $sinh(3\omega)$ is never 0 when $\omega \neq 0$, we see A = 0 also. So the only solution if u is trivial and thats boring so we throw it out.\\
    Case 2: $1 + \Theta = 0$\\
    The model to solve now is
    \begin{eqnarray*}
      u'' = 0\\
      u'(0) = 0\\
      u'(6) = 0
    \end{eqnarray*}
    with characteristic equation $r = 0$ with double root $r = 0$. So the general solution is
    \begin{eqnarray*}
      u(x) = A + Bx
    \end{eqnarray*}
    Applying boundry conditions gives us
    \begin{eqnarray*}
      u(0) = 0\\
      u(6) = 0
    \end{eqnarray*}
    Hence, since $u'(x) = B$, we have
    \begin{eqnarray*}
      u'(0) = 0 = B\\
      u'(6) = 0 = B6
    \end{eqnarray*}
    Hence, B = 0. But the value of A can't be determined. Hence any non zero A gives a nonzero solution.\\
    Choosing A = 1, let $u_0(x) = 1$ be our chosen nonzero. We now need to solve for w in this case. Becuase $\Theta = -1$, the model to solve is\\
    \begin{eqnarray*}
      \frac{dw}{dt} = -\frac{1}{.7}w(t), 0 \leq t
   \end{eqnarray*}
   An the general solution is $w(t) = Ce^{-\frac{1}{.7}t} \; \forall C$. Choosing C = 1 we get 
   \begin{eqnarray*}
    w_0(t) = e^{-\frac{1}{.7}t}
   \end{eqnarray*}
   Hence, the product $\phi_0(x,t) = u_0(x)w_0(t)$ solves the boundary conditions. That is
   \begin{eqnarray*}
    \phi_0(x,t) = e^{-\frac{1}{.7}t}
   \end{eqnarray*}
   is a solution\\
   Case 3: $1 + \Theta = -\omega^2, \omega \neq 0$
   \begin{eqnarray*}
    u(x) = Acos(\frac{\omega}{2}x) +Bsin(\frac{\omega}{2}x)
   \end{eqnarray*}
   and hence
   \begin{eqnarray*}
    u'(x) = -A\frac{\omega}{2}sin(\frac{\omega}{2}x) +B\frac{\omega}{2}cos(\frac{\omega}{2}x)
   \end{eqnarray*}
   Next, apply boundary conditions to find
   \begin{eqnarray*}
    u'(0) = 0 = B\\
    u'(6) = 0 = Asin(3\omega)
   \end{eqnarray*}
   Hence, B = 0 and $Asin(3\omega) = 0$. Thus, we can determine a unieq value for A only if $sin(3\omega) \neq 0$. If $\omega = \frac{n\pi}{3}$ we can solve for A and find A = 0 but other A's cannot be determined. So the only solutions are the trivial or zero solutions unless $\omega 6 = \pi n^2$\\
   \\
   Letting $\omega_n = \frac{n\pi}{3}$, we find a non-zero solution for each nonzero value of A of the form
   \begin{eqnarray*}
    u_n(x) = Acos(\frac{\omega_n}{4}x) = Acos(\frac{n\pi}{6}x)
   \end{eqnarray*}
   For convenience, let's choose all the constants A = 1. Then we have an infinite family of nonzero solutions $u_n(x) = cos(\frac{n\pi}{6}x)$ and an infinite family of separation constants $\Theta_n = -1 - \omega^2_n = -1 0 \frac{n^2\pi^2 4}{36}$\\
   We can solve the w equation. We must solve
   \begin{eqnarray*}
    \frac{dw}{dt} = - \frac{1 + \omega_n^2}{.7}w(t), t \geq 0
   \end{eqnarray*}
   The general solution is
   \begin{eqnarray*}
    w(t) = B_ne^{-\frac{1 + \omega^2_n}{.7}} = B_ne^{-(\frac{1}{.7} + \frac{n^2 \pi^2 4}{(.7)36})t}
   \end{eqnarray*}
   Choosing the constants $B_n = 1$, we obtain the w function\\
   \begin{eqnarray*}
    w_n(t) = e^{-(\frac{1}{.7} + \frac{n^2 \pi^2 4}{(.7)36})t}
   \end{eqnarray*}
   Hence, any product
   \begin{eqnarray*}
    \phi_n(x,t) = u_n(x)w_n(t)
   \end{eqnarray*}
   Will solve the model with the x boundry conditions.\\
   Further, any infinite sum of the form for arbitrary constants $A_n$
   \begin{eqnarray*}
    \Psi_n(x,t) = \sum_{n=1}^N\: A_n\phi_n(x,t) = \sum_{n=1}^N\: A_nu_n(x)w_n(t) = sum_{n=1}^N\: A_ncos(\frac{n\pi}{6})e^{-(\frac{1}{.7} + \frac{n^2 \pi^2 4}{(.7)36})t}
   \end{eqnarray*}
   Adding the $1 + \Theta = 0$ case, we find the most general finite term solution has the form
   \begin{eqnarray*}
    \phi_n(x,t) &=& A_0\Phi_0(x,t) + \sum_{n=1}^\infty\: A_n\phi_n(x,t)\\
    &=& A_0u_0w_0 + \sum_{n=1}^\infty\: A_nu_n(x)w_n(t)\\
    &=& A_0e^{-\frac{1}{.7}} + \sum_{n=1}^\infty\: A_ncos(\frac{n\pi}{6})e^{-(\frac{1}{.7} + \frac{n^2 \pi^2 4}{(.7)36})t} 
   \end{eqnarray*}
   The finite solutions solve the boundry conditions $\frac{\delta \Phi}{\delta x}(0,t) = 0$ and $\frac{\delta \Phi}{\delta x}(6,t) = 0$\\
   For $\Phi(x,0) = f(x)$, we let $n \rightarrow \infty$ and set
   \begin{eqnarray*}
    \Phi(x,t) &=& A_0\Phi_0(x,t) + \sum_{n=1}^\infty\: A_n\phi_n(x,t)\\
    &=& A_0e^{-\frac{1}{.7}t} + \sum_{n=1}^\infty\: A_ncos(\frac{n\pi}{6})e^{-(\frac{1}{.7} + \frac{n^2 \pi^2 4}{(.7)36})t} 
   \end{eqnarray*}
   We take the partial derivative with respect to x of the infinite term and get
   \begin{eqnarray*}
     \sum_{n=1}^\infty\: A_n\frac{n\pi}{6}sin(\frac{n\pi}{6})e^{-(\frac{1}{.7} + \frac{n^2 \pi^2 4}{(.7)36})t} 
   \end{eqnarray*}
   Which satisfies the derivative boundary conditions. So $\Phi(x,t)$ is given by
   \begin{eqnarray*}
    \Phi(x,t) = A_0e^{-\frac{1}{.7}t} + \sum_{n=1}^\infty\: A_ncos(\frac{n\pi}{6}x)e^{-\frac{36 + n^2\pi^2 4}{(.7)36}t}
   \end{eqnarray*}
   For appropriate constants $(A_n)$. We find the right choice of $(A_n)$ comes from
   \begin{eqnarray*}
    \Phi(x,t) = f(x) for 0 \leq x \leq 6
   \end{eqnarray*}
   We know
   \begin{eqnarray*}
    \Phi(x,0) = A_0 + \sum_{n=1}^\infty\: A_ncos(\frac{n\pi}{6}x)
   \end{eqnarray*}
   and so rewriting these in terms of the series solution for $0 \leq x \leq 6$ we find
   \begin{eqnarray*}
    A_0 + \sum_{n=1}^\infty\: A_ncos(\frac{n\pi}{6}x) = f(x)
   \end{eqnarray*}
   The fourier series for the appropriate f is given by
   \begin{eqnarray*}
    f(x) = B + \sum_{n=1}^\infty\: B_ncos(\frac{n\pi}{6}x)
   \end{eqnarray*}
   with
   \begin{eqnarray*}
    B_0 &=& \frac{1}{6}\int_0^6 \: f(x)dx\\
    B_n &=& \frac{1}{3}\int_0^6f(x)cos(\frac{n\pi}{6}x)dx
   \end{eqnarray*}
   Thus setting these series equal, we find a solution given by $A_n = B_n$ for all $n \geq 0$. Thus, we know
   \begin{eqnarray*}
    \Phi(x,t) = B_0 + \sum_{n = 1}^\infty \: B_ncos(\frac{n\pi}{6}x)e^{-\frac{36 + n^2\pi^2 4}{.7(36)}t}
   \end{eqnarray*}
  \end{solution}
\end{exercise}

\end{document}